theories/interrupt/interrupt.thy
@@ -1,0 +1,132 @@
+(*
+
+Copyright (c) 2017, ETH Zurich
+All rights reserved.
+
+Redistribution and use in source and binary forms, with or without
+modification, are permitted provided that the following conditions are met:
+
+1. Redistributions of source code must retain the above copyright notice, this
+   list of conditions and the following disclaimer.
+2. Redistributions in binary form must reproduce the above copyright notice,
+   this list of conditions and the following disclaimer in the documentation
+   and/or other materials provided with the distribution.
+
+THIS SOFTWARE IS PROVIDED BY THE COPYRIGHT HOLDERS AND CONTRIBUTORS "AS IS" AND
+ANY EXPRESS OR IMPLIED WARRANTIES, INCLUDING, BUT NOT LIMITED TO, THE IMPLIED
+WARRANTIES OF MERCHANTABILITY AND FITNESS FOR A PARTICULAR PURPOSE ARE
+DISCLAIMED. IN NO EVENT SHALL THE COPYRIGHT OWNER OR CONTRIBUTORS BE LIABLE FOR
+ANY DIRECT, INDIRECT, INCIDENTAL, SPECIAL, EXEMPLARY, OR CONSEQUENTIAL DAMAGES
+(INCLUDING, BUT NOT LIMITED TO, PROCUREMENT OF SUBSTITUTE GOODS OR SERVICES;
+LOSS OF USE, DATA, OR PROFITS; OR BUSINESS INTERRUPTION) HOWEVER CAUSED AND
+ON ANY THEORY OF LIABILITY, WHETHER IN CONTRACT, STRICT LIABILITY, OR TORT
+(INCLUDING NEGLIGENCE OR OTHERWISE) ARISING IN ANY WAY OUT OF THE USE OF THIS
+SOFTWARE, EVEN IF ADVISED OF THE POSSIBILITY OF SUCH DAMAGE.
+
+*)
+
+(*<*)
+theory interrupt
+  imports Main Set "HOL-Library.Nat_Bijection"  "../model/Model" "../model/Syntax" 
+begin
+(*>*)
+  
+type_synonym PORT = nat
+type_synonym VECTOR = nat
+type_synonym DATA = nat
+type_synonym CONTROLLER_NAME = nat
+  
+datatype FORMAT = FINVALID | FEMPTY | FVECTOR "nat" | FMEMWRITE "nat" "nat"
+  
+record IRQ = 
+  format :: FORMAT
+  port :: PORT
+    
+definition NULL_IRQ :: IRQ
+  where "NULL_IRQ = \<lparr>format = FINVALID, port=0\<rparr>"  
+  
+record CONTROLLER_CLASS =
+  in_port_num :: nat
+  out_port_num :: nat
+  map_valid :: "(IRQ \<Rightarrow> IRQ set) set"
+
+(* Configuration of a controller *)  
+record CONTROLLER =
+  map      :: "IRQ \<Rightarrow> IRQ set"
+ 
+(* Interconnect of the system + each controller with a class *)
+record SYSTEM =
+  controller :: "CONTROLLER_NAME \<Rightarrow> (CONTROLLER \<times> CONTROLLER_CLASS) option"
+  net :: "CONTROLLER_NAME \<Rightarrow> nat \<Rightarrow> (CONTROLLER_NAME \<Rightarrow> nat) set"
+  
+(* look at decoding net to verify *)
+(* assuming system is valid, configuration update \<Rightarrow> system valid *)  
+
+(* Arguments that do not produce an empty set, see dom *)
+definition doms :: "('a \<Rightarrow> 'b set) \<Rightarrow> 'a set" where
+  "doms m = {a. m a \<noteq> {}}"
+  
+(* Get  the actual configuration of a controller name *)   
+definition sys_ctrl_act_conf :: "SYSTEM \<Rightarrow> CONTROLLER_NAME \<Rightarrow> (IRQ \<Rightarrow> IRQ set) option"
+  where "sys_ctrl_act_conf s c = (case controller s c of None \<Rightarrow> None |
+         Some the_c \<Rightarrow> Some (map (fst the_c)))"
+   
+(* Get the set valid configuration of a controller name *)    
+definition sys_ctrl_valid_conf :: "SYSTEM \<Rightarrow> CONTROLLER_NAME \<Rightarrow> ((IRQ \<Rightarrow> IRQ set) set) option"
+  where "sys_ctrl_valid_conf s c = (case controller s c of None \<Rightarrow> None | 
+         Some the_c \<Rightarrow> Some (map_valid (snd the_c)))"
+    
+(* Check if c has a valid config in s *)
+definition sys_ctrl_valid :: "SYSTEM \<Rightarrow> CONTROLLER_NAME \<Rightarrow> bool"
+  where "sys_ctrl_valid s c = (case (sys_ctrl_act_conf s c) of None \<Rightarrow> True | Some conf \<Rightarrow> 
+    case (sys_ctrl_valid_conf s c) of Some valid_confs \<Rightarrow> conf \<in> valid_confs | False)"
+ 
+(* Check if a system is in a valid state *)
+(* valid system = all ports wired, all controller in valid state + ...*)
+definition sys_valid :: "SYSTEM \<Rightarrow> bool"
+  where "sys_valid s = (\<forall> c. c \<in> (dom (controller s)) \<longrightarrow> sys_ctrl_valid s c)"
+
+
+ 
+    
+(* lift to decoding net, assuming valid *)
+    
+(* this does the port+vector/memaddr to natural magic *)
+definition irq_format_nat_encode :: "FORMAT \<Rightarrow> nat" where
+  "irq_format_nat_encode x = (case x of FINVALID \<Rightarrow> prod_encode (0,0) | FEMPTY \<Rightarrow> prod_encode (1,0)
+ | FVECTOR a  \<Rightarrow> prod_encode (2,a) | FMEMWRITE a b \<Rightarrow> prod_encode (3, prod_encode (a,b) ))"
+
+definition irq_format_nat_decode :: "nat \<Rightarrow> FORMAT option" where
+  "irq_format_nat_decode x = (if fst (prod_decode x) = 0 then Some FINVALID else if 
+   fst (prod_decode x) = 1 then Some FEMPTY else if fst (prod_decode x) = 2 then Some (FVECTOR (snd (prod_decode x))) else if
+   fst (prod_decode x) = 3 then Some (FMEMWRITE (fst (prod_decode (snd (prod_decode x)))) (snd (prod_decode (snd (prod_decode x))))) else None)"
+
+
+
+lemma format_enc_inv: "irq_format_nat_decode(irq_format_nat_encode x) = Some x"
+  apply(simp add:irq_format_nat_encode_def add:irq_format_nat_decode_def)
+  by (smt FORMAT.exhaust FORMAT.simps(15) FORMAT.simps(16) FORMAT.simps(17) FORMAT.simps(18) fst_conv numeral_1_eq_Suc_0 numeral_One numeral_eq_iff prod_encode_inverse semiring_norm(83) semiring_norm(86) semiring_norm(89) snd_conv zero_neq_numeral)
+
+definition irq_nat_encode :: "IRQ \<Rightarrow> nat" where
+  "irq_nat_encode i = prod_encode ((irq_format_nat_encode (format i)), port i)"
+
+definition irq_nat_decode :: "nat \<Rightarrow> IRQ option" where
+  "irq_nat_decode n = (case (irq_format_nat_decode (fst (prod_decode n))) of (Some fmt) \<Rightarrow> (Some \<lparr>format = fmt,
+   port = (snd (prod_decode n)) \<rparr> ) | None \<Rightarrow> None)"
+
+lemma "irq_nat_decode(irq_nat_encode x) = Some x"
+  by(simp add:irq_nat_encode_def add:irq_nat_decode_def add:format_enc_inv)
+  
+   
+definition conf_to_translate :: "(IRQ \<Rightarrow> IRQ set) \<Rightarrow> (addr \<Rightarrow> name set)"
+  where "conf_to_translate c = (\<lambda>_. {})"
+    
+definition mk_node :: "SYSTEM \<Rightarrow> CONTROLLER_NAME \<Rightarrow> node"
+  where "mk_node s c = (case (sys_ctrl_act_conf s c) of None \<Rightarrow> empty_node |
+         Some conf \<Rightarrow> \<lparr>accept = {}, translate = conf_to_translate conf \<rparr>)"
+    
+definition mk_net :: "SYSTEM \<Rightarrow> net"
+  where "mk_net s = empty_net"
+    
+  
+end
